lib/FStar.Int32.fst
@@ -28,7 +28,7 @@ let within_int32 (i:int) =
     min_value_int <= i
     && i <= max_value_int
 
-private type int32 =
+abstract type int32 =
   | Int32 : i:int{within_int32 i} -> int32
 
 val min_value : int32
@@ -43,8 +43,8 @@ let as_int (Int32 i) = i
 type nat32 = x:int32{Prims.op_GreaterThanOrEqual (as_int x) 0}
 
 //a ?+ b may overflow
-//must be marked opaque because the body has an intentional admit
-opaque val op_Question_Plus: i:int32
+//must be marked abstract because the body has an intentional admit
+abstract val op_Question_Plus: i:int32
               -> j:int32
               -> Tot (k:int32{within_int32 (as_int i + as_int j) ==> as_int k = as_int i + as_int j})
 let op_Question_Plus (Int32 i) (Int32 j) =
@@ -58,8 +58,8 @@ val op_Plus: i:int32
 let op_Plus (Int32 i) (Int32 j) = Int32 (i + j)
 
 //a ?- b may overflow
-//must be marked opaque because the body has an intentional admit
-opaque val op_Question_Subtraction: i:int32
+//must be marked abstract because the body has an intentional admit
+abstract val op_Question_Subtraction: i:int32
               -> j:int32
               -> Tot (k:int32{within_int32 (as_int i - as_int j) ==> as_int k = as_int i - as_int j})
 let op_Question_Subtraction (Int32 i) (Int32 j) =
@@ -73,8 +73,8 @@ val op_Subtraction: i:int32
 let op_Subtraction (Int32 i) (Int32 j) = Int32 (i - j)
 
 //a ?* b may overflow
-//must be marked opaque because the body has an intentional admit
-opaque val op_Question_Star:
+//must be marked abstract because the body has an intentional admit
+abstract val op_Question_Star:
                  i:int32
               -> j:int32
               -> Tot (k:int32{within_int32 (as_int i * as_int j) ==> as_int k = as_int i * as_int j})
@@ -89,8 +89,8 @@ val op_Star: i:int32
 let op_Star (Int32 i) (Int32 j) = Int32 (i * j)
 
 //When the dividend is negative, the semantics is platform dependent
-//must be marked opaque because the body has an intentional admit
-opaque val op_Question_Slash: i:int32
+//must be marked abstract because the body has an intentional admit
+abstract val op_Question_Slash: i:int32
                            -> j:int32{as_int j <> 0}
                            -> Tot (k:int32{as_int i >= 0 ==> as_int k = as_int i / as_int j})
 let op_Question_Slash (Int32 i) (Int32 j) =
@@ -105,8 +105,8 @@ val op_Slash: i:int32{as_int i >= 0}
 let op_Slash (Int32 i) (Int32 j) = Int32 (i / j)
 
 //a ?% b can overflow
-//must be marked opaque because the body has an intentional admit
-opaque val op_Question_Percent:
+//must be marked abstract because the body has an intentional admit
+abstract val op_Question_Percent:
                 i:int32
              -> j:int32{as_int j <> 0}
              -> Tot (k:int32{not(as_int i = min_value_int && as_int j = -1)
@@ -126,8 +126,8 @@ val op_Percent: i:int32
 let op_Percent (Int32 i) (Int32 j) = Int32 (i % j)
 
 //?- a    can overflow
-//must be marked opaque because the body has an intentional admit
-opaque val op_Question_Minus: i:int32
+//must be marked abstract because the body has an intentional admit
+abstract val op_Question_Minus: i:int32
                    -> Tot int32
 let op_Question_Minus (Int32 i) =
   if i = min_value_int
